coq_ssprove/src/Hacspec_Lib_Pre.v
@@ -36,42 +36,40 @@ Open Scope hacspec_scope.
 Open Scope nat_scope.
 
 Require Import Hacspec_Lib_Comparable.
+From mathcomp Require Import choice.
 
 Section IntType.
 
-  Definition int_choice {WS : wsize} := chWord WS.
-  Definition int_type {WS : wsize} : Type := WS.-word.
-  #[global] Program Instance int {WS : wsize} : ChoiceEquality :=
-    {| ct := @int_choice WS ; T := @int_type WS |}.
+  Definition int {WS : wsize} := chWord WS.
 
-  Definition unsigned {WS : wsize} (i : @int WS) : Z := wunsigned i.
-  Definition signed {WS : wsize} (i: @int WS) : Z := wsigned i.
-  Definition repr {WS : wsize} (z : Z) : @int WS := wrepr WS z.
+  Definition unsigned {WS : wsize} (i : (@int WS)) : Z := wunsigned i.
+  Definition signed {WS : wsize} (i: (@int WS)) : Z := wsigned i.
+  Definition repr {WS : wsize} (z : Z) : (@int WS) := wrepr WS z.
 
-  Definition rol {WS} (u s : @int WS) := wrol u (unsigned s).
-  Definition ror {WS} (u s : @int WS) := wror u (unsigned s).
+  Definition rol {WS} (u s : (@int WS)) := wrol u (unsigned s).
+  Definition ror {WS} (u s : (@int WS)) := wror u (unsigned s).
 
-  #[global] Instance int8 : ChoiceEquality := @int U8.
-  #[global] Instance int16 : ChoiceEquality := @int U16.
-  #[global] Instance int32 : ChoiceEquality := @int U32.
-  #[global] Instance int64 : ChoiceEquality := @int U64.
-  #[global] Instance int128 : ChoiceEquality := @int U128.
+  Definition int8 : choice_type := @int U8.
+  Definition int16 : choice_type := @int U16.
+  Definition int32 : choice_type := @int U32.
+  Definition int64 : choice_type := @int U64.
+  Definition int128 : choice_type := @int U128.
 
-  Definition int_modi {WS : wsize} : @int WS -> @int WS -> @int WS := wmodi.
-  Definition int_add {WS : wsize} : @int WS -> @int WS -> @int WS := @add_word WS.
-  Definition int_sub {WS : wsize} : @int WS -> @int WS -> @int WS := @sub_word WS.
-  Definition int_opp {WS : wsize} : @int WS -> @int WS := @opp_word WS.
-  Definition int_mul {WS : wsize} : @int WS -> @int WS -> @int WS := @mul_word WS.
-  Definition int_div {WS : wsize} : @int WS -> @int WS -> @int WS := wdiv.
-  Definition int_mod {WS : wsize} : @int WS -> @int WS -> @int WS := wmod.
-  Definition int_xor {WS : wsize} : @int WS -> @int WS -> @int WS := wxor.
-  Definition int_and {WS : wsize} : @int WS -> @int WS -> @int WS := wand.
-  Definition int_or {WS : wsize} : @int WS -> @int WS -> @int WS := wor.
+  Definition int_modi {WS : wsize} : (@int WS) -> (@int WS) -> (@int WS) := wmodi.
+  Definition int_add {WS : wsize} : (@int WS) -> (@int WS) -> (@int WS) := @add_word WS.
+  Definition int_sub {WS : wsize} : (@int WS) -> (@int WS) -> (@int WS) := @sub_word WS.
+  Definition int_opp {WS : wsize} : (@int WS) -> (@int WS) := @opp_word WS.
+  Definition int_mul {WS : wsize} : (@int WS) -> (@int WS) -> (@int WS) := @mul_word WS.
+  Definition int_div {WS : wsize} : (@int WS) -> (@int WS) -> (@int WS) := wdiv.
+  Definition int_mod {WS : wsize} : (@int WS) -> (@int WS) -> (@int WS) := wmod.
+  Definition int_xor {WS : wsize} : (@int WS) -> (@int WS) -> (@int WS) := wxor.
+  Definition int_and {WS : wsize} : (@int WS) -> (@int WS) -> (@int WS) := wand.
+  Definition int_or {WS : wsize} : (@int WS) -> (@int WS) -> (@int WS) := wor.
 
-  Definition int_not {WS : wsize} : @int WS -> @int WS := wnot.
+  Definition int_not {WS : wsize} : (@int WS) -> (@int WS) := wnot.
 
-  Definition zero {WS : wsize} : T (@int WS) := @word0 WS.
-  Definition one {WS : wsize} : T (@int WS) := @word1 (pred WS).
+  Definition zero {WS : wsize} : (@int WS) := @word0 WS.
+  Definition one {WS : wsize} : (@int WS) := @word1 (pred WS).
 
   Lemma add_zero_l : forall {WS : wsize} n, @int_add WS zero n = n.
   Proof.
@@ -131,7 +129,7 @@ Section IntType.
 
 End IntType.
 
-Axiom secret : forall {WS : wsize},  (T (@int WS)) -> (T (@int WS)).
+Axiom secret : forall {WS : wsize},  ((@int WS)) -> ((@int WS)).
 
 Infix "%%" := int_modi (at level 40, left associativity) : Z_scope.
 Infix ".+" := int_add (at level 77) : hacspec_scope.
@@ -184,81 +182,81 @@ Global Instance Z_comparable : Comparable Z := {
     geb a b := Z.leb b a;
   }.
 
-Lemma int_eqb_eq : forall {WS : wsize} (a b : @int WS), eqtype.eq_op a b = true <-> a = b.
+Lemma int_eqb_eq : forall {WS : wsize} (a b : (@int WS)), eqtype.eq_op a b = true <-> a = b.
 Proof.
   symmetry ; exact (ssrbool.rwP (@eqtype.eqP _ a b)).
 Qed.
 
-Global Instance int_eqdec `{WS : wsize}: EqDec (@int WS) := {
+Global Instance int_eqdec `{WS : wsize}: EqDec ((@int WS)) := {
     eqb := eqtype.eq_op;
     eqb_leibniz := int_eqb_eq ;
   }.
 
-Global Instance int_comparable `{WS : wsize} : Comparable (@int WS) :=
+Global Instance int_comparable `{WS : wsize} : Comparable ((@int WS)) :=
   eq_dec_lt_Comparable (wlt Unsigned).
 
-Axiom uint8_declassify : int8 -> int8.
-Axiom int8_declassify : int8 -> int8.
-Axiom uint16_declassify : int16 -> int16.
-Axiom int16_declassify : int16 -> int16.
-Axiom uint32_declassify : int32 -> int32.
-Axiom int32_declassify : int32 -> int32.
-Axiom uint64_declassify : int64 -> int64.
-Axiom int64_declassify : int64 -> int64.
-Axiom uint128_declassify : int128 -> int128.
-Axiom int128_declassify : int128 -> int128.
+Axiom uint8_declassify : (int8) -> (int8).
+Axiom int8_declassify : (int8) -> (int8).
+Axiom uint16_declassify : (int16) -> (int16).
+Axiom int16_declassify : (int16) -> (int16).
+Axiom uint32_declassify : (int32) -> (int32).
+Axiom int32_declassify : (int32) -> (int32).
+Axiom uint64_declassify : (int64) -> (int64).
+Axiom int64_declassify : (int64) -> (int64).
+Axiom uint128_declassify : (int128) -> (int128).
+Axiom int128_declassify : (int128) -> (int128).
 
-Axiom uint8_classify : int8 -> int8.
-Axiom int8_classify : int8 -> int8.
-Axiom uint16_classify : int16 -> int16.
-Axiom int16_classify : int16 -> int16.
-Axiom uint32_classify : int32 -> int32.
-Axiom int32_classify : int32 -> int32.
-Axiom uint64_classify : int64 -> int64.
-Axiom int64_classify : int64 -> int64.
-Axiom uint128_classify : int128 -> int128.
-Axiom int128_classify : int128 -> int128.
+Axiom uint8_classify : (int8) -> (int8).
+Axiom int8_classify : (int8) -> (int8).
+Axiom uint16_classify : (int16) -> (int16).
+Axiom int16_classify : (int16) -> (int16).
+Axiom uint32_classify : (int32) -> (int32).
+Axiom int32_classify : (int32) -> (int32).
+Axiom uint64_classify : (int64) -> (int64).
+Axiom int64_classify : (int64) -> (int64).
+Axiom uint128_classify : (int128) -> (int128).
+Axiom int128_classify : (int128) -> (int128).
 
 
 (* CompCert integers' signedness is only interpreted through 'signed' and 'unsigned',
    and not in the representation. Therefore, uints are just names for their respective ints.
  *)
 
-Definition int8_type := @int_type U8.
-Definition int16_type := @int_type U16.
-Definition int32_type := @int_type U32.
-Definition int64_type := @int_type U64.
-Definition int128_type := @int_type U128.
+(* Definition int8_type := (@int U8). *)
+(* Definition int16_type := (@int U16). *)
+(* Definition int32_type := (@int U32). *)
+(* Definition int64_type := (@int U64). *)
+(* Definition int128_type := (@int U128). *)
 
 Notation uint8 := int8.
-Definition uint8_type := @int_type U8.
-#[global] Instance uint16 : ChoiceEquality := int16.
-Definition uint16_type := @int_type U16.
-#[global] Instance uint32 : ChoiceEquality := int32.
-Definition uint32_type := @int_type U32.
-#[global] Instance uint64 : ChoiceEquality := int64.
-Definition uint64_type := @int_type U64.
-#[global] Instance uint128 : ChoiceEquality := int128.
-Definition uint128_type := @int_type U128.
+(* Definition uint8_type := (@int U8). *)
+Definition uint16 : choice_type := int16.
+(* Definition uint16_type := (@int U16). *)
+Definition uint32 : choice_type := int32.
+(* Definition uint32_type := (@int U32). *)
+Definition uint64 : choice_type := int64.
+(* Definition uint64_type := (@int U64). *)
+Definition uint128 : choice_type := int128.
+(* Definition uint128_type := (@int U128). *)
 
-#[global] Instance uint_size : ChoiceEquality := int32.
-Definition uint_size_type := @int_type U32.
+Definition uint_size : choice_type := int32.
+(* Definition uint_size_type := @int_type U32. *)
 
-#[global] Instance int_size : ChoiceEquality := int32.
-Definition int_size_type := @int_type U32.
+Definition int_size : choice_type := int32.
+(* Definition int_size_type := @int_type U32. *)
 
-Axiom declassify_usize_from_uint8 : uint8 -> uint_size.
-Axiom declassify_u32_from_uint32 : uint32 -> uint32.
+Axiom declassify_usize_from_uint8 : (uint8) -> (uint_size).
+Axiom declassify_u32_from_uint32 : (uint32) -> (uint32).
 
 (* Represents any type that can be converted to uint_size and back *)
 Class UInt_sizeable (A : Type) := {
-    usize : A -> uint_size;
-    from_uint_size : uint_size -> A;
+    usize : A -> (uint_size);
+    from_uint_size : (uint_size) -> A;
   }.
 Arguments usize {_} {_}.
 Arguments from_uint_size {_} {_}.
 
-Identity Coercion uint_size_to_int:uint_size_type >-> int_type.
+(* Identity Coercion usize:>-> nat. *)
 
 Global Instance nat_uint_sizeable : UInt_sizeable nat := {
     usize n := repr (Z.of_nat n);
@@ -357,10 +355,10 @@ Infix "usize_shift_left" := (usize_shift_left) (at level 77) : hacspec_scope.
 Definition pub_uint128_wrapping_add (x y: int128) : int128 :=
   x .+ y.
 
-Definition shift_left_ `{WS : wsize} (i : @int WS) (j : uint_size) : @int WS :=
+Definition shift_left_ `{WS : wsize} (i : (@int WS)) (j : uint_size) : (@int WS) :=
   wshl i (@repr WS (from_uint_size j)).
 
-Definition shift_right_ `{WS : wsize} (i : @int WS) (j : uint_size) : @int WS:=
+Definition shift_right_ `{WS : wsize} (i : (@int WS)) (j : uint_size) : (@int WS):=
   wshr i (@repr WS (from_uint_size j)) .
 
 Infix "shift_left" := (shift_left_) (at level 77) : hacspec_scope.
@@ -724,11 +722,11 @@ Proof.
 Qed.
 
 Lemma foldi__nat_move_to_function :
-  forall {acc: ChoiceEquality}
+  forall {acc: choice_type}
          (fuel : nat)
          (i : nat)
          (f : nat -> acc -> acc)
-         (cur : T acc),
+         (cur : acc),
     foldi_nat_ fuel i (fun x => f (S x)) (cur) = foldi_nat_ fuel (S i) f cur.
 Proof.
   induction fuel ; intros.
@@ -739,11 +737,11 @@ Proof.
 Qed.
 
 Lemma foldi__nat_move_to_function_add :
-  forall {acc: ChoiceEquality}
+  forall {acc: choice_type}
          (fuel : nat)
          (i j : nat)
-         (f : nat -> T acc ->  acc)
-         (cur : T acc),
+         (f : nat -> acc ->  acc)
+         (cur : acc),
     foldi_nat_ fuel i (fun x => f (x + j)%nat) (cur) = foldi_nat_ fuel (i + j) f cur.
 Proof.
   intros acc fuel i j. generalize dependent i.
@@ -765,7 +763,7 @@ Proof.
 Qed.
 
 Theorem foldi_for_loop_range_eq :
-  forall {acc : ChoiceEquality} lo hi f (cur : acc),
+  forall {acc : choice_type} lo hi f (cur : acc),
     foldi_nat lo hi f cur
     =
       for_loop_range lo hi f cur.
@@ -1021,52 +1019,55 @@ Qed.
 
 (*** Seq *)
 
-Definition nseq_choice (A: ChoiceEquality) (len : nat) : choice_type :=
+Definition nseq' (A: choice_type) (len : nat) : choice_type :=
   match len with
   | O => chUnit (* A *)
-  | S n => chMap ('fin (S n)) (ct A)
+  | S n => chMap ('fin (S n)) (A)
   end.
 
-Definition nseq_type (A: ChoiceEquality) (len : nat) : Type :=
+Definition nseq (A: choice_type) (len : uint_size) : choice_type :=
+  nseq' A (Z.to_nat (unsigned len)).
+
+Definition nseq_type (A: choice_type) (len : nat) : Type :=
   match len with
   | 0%nat => unit
-  | S n => fmap.FMap.fmap_type (ordinal_ordType len) (T _)
+  | S n => fmap.FMap.fmap_type (ordinal_ordType len) (A)
   end.
 
-#[global] Program Instance nseq (A: ChoiceEquality) (len : nat) : ChoiceEquality :=
-  {| ct := nseq_choice A len ; T := nseq_type A len |}.
-Next Obligation.
-  intros.
-  unfold nseq_type.
-  unfold nseq_choice.
-  rewrite <- @ChoiceEq.
-  destruct (len) ; reflexivity.
-Defined.
+(* #[global] Program Instance nseq (A: choice_type) (len : nat) : choice_type := *)
+(*   {| ct := nseq_choice A len ; T := nseq_type A len |}. *)
+(* Next Obligation. *)
+(*   intros. *)
+(*   unfold nseq_type. *)
+(*   unfold nseq_choice. *)
+(*   rewrite <- @ChoiceEq. *)
+(*   destruct (len) ; reflexivity. *)
+(* Defined. *)
 
-Definition seq_choice (A : ChoiceEquality) : choice_type := chMap 'nat (ct A).
-Definition seq_type (A : ChoiceEquality) : Type := FMap.fmap_type nat_ordType (T _).
-Program Definition seq (A : ChoiceEquality) : ChoiceEquality :=
-  {| ct := seq_choice A ; T := seq_type A ; |}.
-Next Obligation.
-  intros.
-  unfold seq_type.
-  rewrite <- @ChoiceEq.
-  reflexivity.
-Defined.
+Definition seq (A : choice_type) : choice_type := chMap 'nat A.
+Definition seq_type (A : choice_type) : Type := FMap.fmap_type nat_ordType (A).
+(* Program Definition seq (A : choice_type) : choice_type := *)
+(*   {| ct := seq_choice A ; T := seq_type A ; |}. *)
+(* Next Obligation. *)
+(*   intros. *)
+(*   unfold seq_type. *)
+(*   rewrite <- @ChoiceEq. *)
+(*   reflexivity. *)
+(* Defined. *)
 
 Definition public_byte_seq := seq int8.
 Definition byte_seq := seq int8.
 Definition list_len := length.
 
-Definition seq_index {A: ChoiceEquality} `{Default (T A)} (s: T (seq A)) (i : uint_size) : T A :=
+Definition seq_index {A: choice_type} `{Default (A)} (s: (seq A)) (i : uint_size) : A :=
   match getm s (from_uint_size i) with
   | Some a => a
   | None => default
   end.
 
-Definition seq_len {A: ChoiceEquality} (s: T (seq A)) : T (uint_size) := usize (length s).
+Definition seq_len {A: choice_type} (s: (seq A)) : (uint_size) := usize (length s).
 
-Definition seq_to_list (A: ChoiceEquality) (s : T (seq A)) : list (T A).
+Definition seq_to_list (A: choice_type) (s : (seq A)) : list (A).
 Proof.
   apply @FMap.fmval in s ; fold chElement in s.
   induction s.
@@ -1076,17 +1077,17 @@ Proof.
     apply (s0 :: IHs).
 Defined.
 
-Definition seq_from_list (A : ChoiceEquality) (l : list (T A)) : T (seq A) :=
+Definition seq_from_list (A : choice_type) (l : list ( A)) :  (seq A) :=
   fmap_of_seq l.
 
 
-Definition seq_new_ {A: ChoiceEquality} (init : A) (len: nat) : seq A :=
+Definition seq_new_ {A: choice_type} (init : A) (len: nat) : (seq A) :=
   fmap_of_seq (repeat init len).
 
-Definition seq_new {A: ChoiceEquality} `{Default A} (len: nat) : seq A :=
+Definition seq_new {A: choice_type} `{Default (A)} (len: nat) : (seq A) :=
   seq_new_ default len.
 
-Definition seq_create {A: ChoiceEquality} `{Default A} (len: nat) : seq A :=
+Definition seq_create {A: choice_type} `{Default (A)} (len: nat) : (seq A) :=
   seq_new len.
 
 Fixpoint list_iter (n : nat) (k : nat) `{(n <= k)%nat} : list { x : nat | (x < k)%nat }.
@@ -1109,48 +1110,49 @@ Proof.
 Qed.
 
 Definition array_from_list
-           (A: ChoiceEquality)
-           (l: list (T A))
-  : T (nseq A (length l)).
+           (A: choice_type)
+           (l: list ( A))
+  :  (nseq' A (length l)).
 Proof.
   destruct l as [ | x xs ].
   - apply tt.
   - pose (l := x :: xs).
-    pose proof (seq.foldr (fun (x : (T A) * { x : nat | (x < length l)%nat }) y =>
+    pose proof (seq.foldr (fun (x : (A) * { x : nat | (x < length l)%nat }) y =>
                              setm
-                               (S := (T A))
+                               (S := (A))
                                y
                                (fintype.Ordinal (n := length l) (m := proj1_sig (snd x)) (ssrbool.introT ssrnat.ltP (proj2_sig (snd x))))
                                (fst x))
                           emptym
                           (seq.zip l (@list_iter (length l) (length l) (le_n (length l))))).
-    rewrite <- ChoiceEq.
-    hnf.
-    rewrite ChoiceEq.
+    (* rewrite <- ChoiceEq. *)
+    (* hnf. *)
+    (* rewrite ChoiceEq. *)
     apply X.
 Defined.
 
 (**** Array manipulation *)
 
 
-Definition array_new_ {A: ChoiceEquality} (init:T A) (len: nat) : T (nseq A len).
-  unfold T.
+Definition array_new_ {A: choice_type} (init:A) (len: uint_size) : (nseq A len).
+  (* unfold T. *)
   unfold nseq.
-  rewrite <- (repeat_length init (len)).
+  unfold nseq'.
+  rewrite <- (repeat_length init (Z.to_nat (unsigned len))).
   intros.
-  apply (@array_from_list A (repeat init len)).
+  apply (@array_from_list A (repeat init (Z.to_nat (unsigned len)))).
 Defined.
 
 
-Definition array_index {A: ChoiceEquality} `{Default (T A)} {len : nat} (s: T (nseq A len)) {WS} (i: @int WS) : T A.
+Definition array_index {A: choice_type} `{Default (A)} {len : nat} (s: (nseq' A len)) {WS} (i: (@int WS)) : A.
 Proof.
   destruct (Z.to_nat (unsigned i) <? len)%nat eqn:H1.
   (* If i < len, index normally *)
   - apply Nat.ltb_lt in H1.
     destruct len. { lia. }
-    rewrite <- ChoiceEq in s.
+    (* rewrite <- ChoiceEq in s. *)
     cbn in s.
-    rewrite -> ChoiceEq in s.
+    (* rewrite -> ChoiceEq in s. *)
     destruct (@getm _ _ s (fintype.Ordinal (n := S len) (m := Z.to_nat (unsigned i)) (ssrbool.introT ssrnat.ltP H1))) as [f | ].
     + exact f.
     + exact default.
@@ -1160,18 +1162,18 @@ Proof.
 Defined.
 
 
-Definition array_upd {A: ChoiceEquality} {len : nat} (s: T (nseq A len)) {WS} (i: @int WS) (new_v: T A) : T (nseq A len).
+Definition array_upd {A: choice_type} {len : nat} (s: (nseq' A len)) {WS} (i: (@int WS)) (new_v: A) : (nseq' A len).
 Proof.
   destruct (Z.to_nat (unsigned i) <? len)%nat eqn:v.
   (* If i < len, update normally *)
   - apply Nat.ltb_lt in v.
     destruct len. { lia. }
-    rewrite <- ChoiceEq in s.
+    (* rewrite <- ChoiceEq in s. *)
     cbn in s.
-    rewrite -> ChoiceEq in s.
-    rewrite <- ChoiceEq.
+    (* rewrite -> ChoiceEq in s. *)
+    (* rewrite <- ChoiceEq. *)
     cbn.
-    rewrite -> ChoiceEq.
+    (* rewrite -> ChoiceEq. *)
     apply (setm s (fintype.Ordinal (m := Z.to_nat (unsigned i)) (ssrbool.introT ssrnat.ltP v)) new_v).
   (* otherwise return original array *)
   - exact s.
@@ -1180,7 +1182,7 @@ Defined.
 (* Definition array_upd {A: Type} {len : uint_size} (s: lseq A len) (i: uint_size) (new_v: A) : lseq A len := List.upd s i new_v. *)
 
 (* substitutes a sequence (nseq) into an array (nseq), given index interval  *)
-Definition update_sub {A : ChoiceEquality} {len slen} `{Default (T A)} (v : T (nseq A len)) (i : nat) (n : nat) (sub : T (nseq A slen)) : T (nseq A len) :=
+Definition update_sub {A : choice_type} {len slen} `{Default (A)} (v : (nseq' A len)) (i : nat) (n : nat) (sub : (nseq' A slen)) : (nseq' A len) :=
   let fix rec x acc :=
     match x with
     | 0%nat => acc
@@ -1192,20 +1194,20 @@ Definition update_sub {A : ChoiceEquality} {len slen} `{Default (T A)} (v : T (n
 (* Compute (to_list (update_sub [1;2;3;4;5] 0 4 (of_list [9;8;7;6;12]))). *)
 
 Definition array_from_seq
-           {a: ChoiceEquality}
-           `{Default (T a)}
-           (out_len:nat)
+           {a: choice_type}
+           `{Default (a)}
+           (out_len:uint_size)
            (input: seq_type a)
-  : T (nseq a out_len) :=
-  let out := array_new_ default out_len in
-  update_sub out 0 (out_len - 1) (@array_from_list a (@seq_to_list a input)).
+  : (nseq a out_len) :=
+  let out := array_new_ default (out_len) in
+  update_sub out 0 ((Z.to_nat (unsigned out_len)) - 1) (@array_from_list a (@seq_to_list a input)).
 
 (* Global Coercion array_from_seq : seq_type >-> nseq_type. *)
 
 Definition slice {A} (l : list A) (i j : nat) : list A :=
   if (j <=? i)%nat then [] else firstn (j-i+1) (skipn i l).
 
-Fixpoint array_to_list_helper {A : ChoiceEquality} {n} (f : T (nseq A (S n))) (i : nat) `{(i < S (S n))%nat} : list (T A).
+Fixpoint array_to_list_helper {A : choice_type} {n} (f : (nseq' A (S n))) (i : nat) `{(i < S (S n))%nat} : list (A).
   destruct i as [ | i' ].
   - exact [].
   - refine match getm f (fintype.Ordinal (m := i') _) with
@@ -1213,21 +1215,22 @@ Fixpoint array_to_list_helper {A : ChoiceEquality} {n} (f : T (nseq A (S n))) (i
            | Some a => array_to_list_helper A n f i' _ ++ [a]
            end.
     + apply (ssrbool.introT ssrnat.ltP).
+      cbn.
       lia.
     + lia.
 Defined.
 
-Definition array_to_list {A : ChoiceEquality} {n} (f : T (nseq A n)) : list (T A).
+Definition array_to_list {A : choice_type} {n} (f : (nseq' A n)) : list (A).
   destruct n.
   - apply [].
   - refine (array_to_list_helper f (S n) (H := _)).
     lia.
 Defined.
 
-Definition array_to_seq {A : ChoiceEquality} {n} (f : nseq_type A n) : seq_type _ :=
+Definition array_to_seq {A : choice_type} {n} (f : (nseq' A n)) : seq_type _ :=
   seq_from_list _ (array_to_list f).
 
-Definition positive_slice {A : ChoiceEquality} `{Hd: Default (T A)} {n} `{H: Positive n} (l : T (nseq A n)) (i j : nat) `{H1: (i < j)%nat} `{(j - i < length (array_to_list l) - i)%nat} : Positive (length (slice (array_to_list l) i j)).
+Definition positive_slice {A : choice_type} `{Hd: Default (A)} {n} `{H: Positive n} (l : (nseq' A n)) (i j : nat) `{H1: (i < j)%nat} `{(j - i < length (array_to_list l) - i)%nat} : Positive (length (slice (array_to_list l) i j)).
 Proof.
   unfold slice.
   rewrite (proj2 (Nat.leb_gt j i) H1).
@@ -1252,213 +1255,213 @@ Proof.
   - reflexivity.
 Qed.
 
-Definition lseq_slice {A : ChoiceEquality} {n} (l : T (nseq A n)) (i j : nat) :
-  T (@nseq A (length (slice (array_to_list l) (i) (j)))) :=
+Definition lseq_slice {A : choice_type} {n} (l : (nseq A n)) (i j : nat) :
+  (@nseq' A (length (slice (array_to_list l) (i) (j)))) :=
   array_from_list _ (slice (array_to_list l) (i) (j)).
 
-Definition seq_sub {a : ChoiceEquality} `{Default (T (a))} (s : (T (seq a))) (start n : nat) :=
-  lseq_slice (array_from_seq (from_uint_size (seq_len s)) s) start (start + n)%nat.
+Definition seq_sub {a : choice_type} `{Default ((a))} (s : ((seq a))) (start n : nat) :=
+  lseq_slice (array_from_seq (seq_len s) s) start (start + n)%nat.
 
 Definition array_update_slice
-           {a : ChoiceEquality}
-           `{Default (T (a))}
+           {a : choice_type}
+           `{Default ((a))}
            {l : nat}
-           (out: (T (nseq a l)))
+           (out: ((nseq' a l)))
            (start_out: nat)
-           (input: (T (seq a)))
+           (input: ((seq a)))
            (start_in: nat)
            (len: nat)
-  : (T (nseq a l)) :=
+  : ((nseq' a l)) :=
   update_sub out start_out (len) (seq_sub input start_in len).
 
 Definition array_from_slice
-           {a: ChoiceEquality}
-           `{Default (T a)}
-           (default_value: (T a))
-           (out_len: nat)
-           (input: T (seq a))
-           (start: nat)
-           (slice_len: nat)
-  : T (nseq a out_len) :=
+           {a: choice_type}
+           `{Default (a)}
+           (default_value: (a))
+           (out_len: uint_size)
+           (input: (seq a))
+           (start: uint_size)
+           (slice_len: uint_size)
+  : (nseq a out_len) :=
   let out := array_new_ default out_len in
   array_from_seq out_len input.
 
 Definition array_slice
-           {a: ChoiceEquality}
-           `{Default (T a)}
-           (input: T (seq a))
+           {a: choice_type}
+           `{Default (a)}
+           (input: (seq a))
            (start: nat)
-           (slice_len: nat)
-  : T (nseq a slice_len) :=
+           (slice_len: uint_size)
+  : (nseq a slice_len) :=
   array_from_slice default (slice_len) input (slice_len) (slice_len).
 
 Definition array_from_slice_range
-           {a: ChoiceEquality}
-           `{Default (T a)}
-           (default_value: T a)
-           (out_len: nat)
-           (input: T (seq a))
-           (start_fin: (T uint_size * T uint_size))
-  : T (nseq a out_len).
+           {a: choice_type}
+           `{Default (a)}
+           (default_value: a)
+           (out_len: uint_size)
+           (input: (seq a))
+           (start_fin: (uint_size * uint_size))
+  : (nseq a out_len).
 Proof.
   pose (out := array_new_ default_value (out_len)).
   destruct start_fin as [start fin].
   refine (update_sub out 0 ((from_uint_size fin) - (from_uint_size start)) _).
 
-  apply (@lseq_slice a ((from_uint_size fin) - (from_uint_size start)) (array_from_seq ((from_uint_size fin) - (from_uint_size start)) input) (from_uint_size start) (from_uint_size fin)).
+  apply (@lseq_slice a (fin .- start) (array_from_seq (fin .- start) input) (from_uint_size start) (from_uint_size fin)).
 Defined.
 
 Definition array_slice_range
-           {a: ChoiceEquality}
-           `{Default (T a)}
+           {a: choice_type}
+           `{Default (a)}
            {len : nat}
-           (input: T (nseq a len))
-           (start_fin:(T uint_size * T uint_size))
-  : T (seq a) :=
+           (input: (nseq a (usize len)))
+           (start_fin:(uint_size * uint_size))
+  : (seq a) :=
   array_to_seq (lseq_slice input (from_uint_size (fst start_fin)) (from_uint_size (snd start_fin))).
 
 Definition array_update
-           {a: ChoiceEquality}
-           `{Default (T a)}
+           {a: choice_type}
+           `{Default (a)}
            {len: nat}
-           (s: T (nseq a len))
+           (s: (nseq' a len))
            (start : nat)
-           (start_s: T (seq a))
-  : T (nseq a len) :=
-  update_sub s start (from_uint_size (seq_len start_s)) (array_from_seq (from_uint_size (seq_len start_s)) (start_s)).
+           (start_s: (seq a))
+  : (nseq' a len) :=
+  update_sub s start (from_uint_size (seq_len start_s)) (array_from_seq ((seq_len start_s)) (start_s)).
 
 Definition array_update_start
-           {a: ChoiceEquality}
-           `{Default (T a)}
+           {a: choice_type}
+           `{Default (a)}
            {len: nat}
-           (s: T (nseq a len))
-           (start_s: T (seq a))
-  : T (nseq a len) :=
-  update_sub s 0 (from_uint_size (seq_len start_s)) (array_from_seq (from_uint_size (seq_len start_s)) start_s).
+           (s: (nseq' a len))
+           (start_s: (seq a))
+  : (nseq' a len) :=
+  update_sub s 0 (from_uint_size (seq_len start_s)) (array_from_seq ((seq_len start_s)) start_s).
 
 
-Definition array_len  {a: ChoiceEquality} {len: nat} (s: T (nseq a len)) : uint_size := usize len.
+Definition array_len  {a: choice_type} {len: nat} (s: (nseq' a len)) : uint_size := usize len.
 (* May also come up as 'length' instead of 'len' *)
-Definition array_length  {a: ChoiceEquality} {len: nat} (s: T (nseq a len)) : uint_size := usize len.
+Definition array_length  {a: choice_type} {len: nat} (s: (nseq' a len)) : uint_size := usize len.
 
 (**** Seq manipulation *)
 
 Definition seq_slice
-           {a: ChoiceEquality}
-           `{Default (T a)}
-           (s: (T (seq a)))
-           (start: T (uint_size))
-           (len: T (uint_size))
+           {a: choice_type}
+           `{Default (a)}
+           (s: ((seq a)))
+           (start: (uint_size))
+           (len: (uint_size))
   : (seq a) :=
-  array_to_seq (lseq_slice (array_from_seq (from_uint_size (seq_len s)) s) (from_uint_size start) ((from_uint_size start) + (from_uint_size len))).
+  array_to_seq (lseq_slice (array_from_seq ((seq_len s)) s) (from_uint_size start) ((from_uint_size start) + (from_uint_size len))).
 
 Definition seq_slice_range
-           {a: ChoiceEquality}
-           `{Default (T (a))}
-           (input: (T (seq a)))
-           (start_fin:((T (uint_size)) * (T (uint_size))))
-  : (T (seq a)) :=
+           {a: choice_type}
+           `{Default ((a))}
+           (input: ((seq a)))
+           (start_fin:(((uint_size)) * ((uint_size))))
+  : ((seq a)) :=
   seq_slice input (fst start_fin) (snd start_fin).
 
 (* updating a subsequence in a sequence *)
 Definition seq_update
-           {a: ChoiceEquality}
-           `{Default (T (a))}
-           (s: (T (seq a)))
+           {a: choice_type}
+           `{Default ((a))}
+           (s: ((seq a)))
            (start: uint_size)
-           (input: (T (seq a)))
-  : (T (seq a)) :=
-  array_to_seq (update_sub (array_from_seq (from_uint_size (seq_len s)) s) (from_uint_size start) (from_uint_size (seq_len input)) (array_from_seq (from_uint_size (seq_len input)) input)).
+           (input: ((seq a)))
+  : ((seq a)) :=
+  array_to_seq (update_sub (array_from_seq ((seq_len s)) s) (from_uint_size start) (from_uint_size (seq_len input)) (array_from_seq ( (seq_len input)) input)).
 
 (* updating only a single value in a sequence*)
 Definition seq_upd
-           {a: ChoiceEquality}
-           `{Default (T (a))}
-           (s: (T (seq a)))
+           {a: choice_type}
+           `{Default ((a))}
+           (s: ((seq a)))
            (start: uint_size)
-           (v: (T (a)))
-  : (T (seq a)) :=
+           (v: ((a)))
+  : ((seq a)) :=
   seq_update s start (setm emptym 0%nat v).
 
 Definition seq_update_start
-           {a: ChoiceEquality}
-           `{Default (T (a))}
-           (s: (T (seq a)))
-           (start_s: (T (seq a)))
-  : (T (seq a)) :=
-  array_to_seq (update_sub (array_from_seq (from_uint_size (seq_len s)) s) 0 (from_uint_size (seq_len start_s)) (array_from_seq (from_uint_size (seq_len start_s)) start_s)).
+           {a: choice_type}
+           `{Default ((a))}
+           (s: ((seq a)))
+           (start_s: ((seq a)))
+  : ((seq a)) :=
+  array_to_seq (update_sub (array_from_seq ((seq_len s)) s) 0 (from_uint_size (seq_len start_s)) (array_from_seq ((seq_len start_s)) start_s)).
 
 Definition seq_update_slice
-           {a : ChoiceEquality}
-           `{Default (T (a))}
-           (out: (T (seq a)))
+           {a : choice_type}
+           `{Default ((a))}
+           (out: ((seq a)))
            (start_out: nat)
-           (input: (T (seq a)))
+           (input: ((seq a)))
            (start_in: nat)
            (len: nat)
-  : (T (seq a))
+  : ((seq a))
   :=
-  array_to_seq (update_sub (array_from_seq (from_uint_size (seq_len out)) out) start_out len (seq_sub input start_in len)).
+  array_to_seq (update_sub (array_from_seq ((seq_len out)) out) start_out len (seq_sub input start_in len)).
 
 Definition seq_concat
-           {a : ChoiceEquality}
-           (s1 :(T (seq a)))
-           (s2: (T (seq a)))
-  : (T (seq a)) :=
+           {a : choice_type}
+           (s1 :((seq a)))
+           (s2: ((seq a)))
+  : ((seq a)) :=
   seq_from_list _ (seq_to_list _ s1 ++ seq_to_list _ s2).
 
 Definition seq_concat_owned
-           {a : ChoiceEquality}
-           (s1 :(T (seq a)))
-           (s2: (T (seq a)))
-  : (T (seq a)) := seq_concat s1 s2.
+           {a : choice_type}
+           (s1 :((seq a)))
+           (s2: ((seq a)))
+  : ((seq a)) := seq_concat s1 s2.
 
 Definition seq_push
-           {a : ChoiceEquality}
-           (s1 :(T (seq a)))
-           (s2: (T (a)))
-  : (T (seq a)) :=
+           {a : choice_type}
+           (s1 :((seq a)))
+           (s2: ((a)))
+  : ((seq a)) :=
   seq_from_list _ ((seq_to_list _ s1) ++ [s2]).
 
 Definition seq_push_owned
-           {a : ChoiceEquality}
-           (s1 :(T (seq a)))
-           (s2: (T (a)))
-  : (T (seq a)) := seq_push s1 s2.
+           {a : choice_type}
+           (s1 :((seq a)))
+           (s2: ((a)))
+  : ((seq a)) := seq_push s1 s2.
 
 Definition seq_from_slice
-           {a: ChoiceEquality}
-           `{Default (T (a))}
-           (input: (T (seq a)))
-           (start_fin: ((T (uint_size)) * (T (uint_size))))
-  : (T (seq a)) :=
-  let out := array_new_ (default) (from_uint_size (seq_len input)) in
+           {a: choice_type}
+           `{Default ((a))}
+           (input: ((seq a)))
+           (start_fin: (((uint_size)) * ((uint_size))))
+  : ((seq a)) :=
+  let out := array_new_ (default) ((seq_len input)) in
   let (start, fin) := start_fin in
-  array_to_seq (update_sub out 0 ((from_uint_size fin) - (from_uint_size start)) ((lseq_slice (array_from_seq (from_uint_size (seq_len input)) input) (from_uint_size start) (from_uint_size fin)))).
+  array_to_seq (update_sub out 0 ((from_uint_size fin) - (from_uint_size start)) ((lseq_slice (array_from_seq ( (seq_len input)) input) (from_uint_size start) (from_uint_size fin)))).
 
 Definition seq_from_slice_range
-           {a: ChoiceEquality}
-           `{Default (T (a))}
-           (input: (T (seq a)))
-           (start_fin: ((T (uint_size)) * (T (uint_size))))
-  : (T (seq a)) :=
-  let out := array_new_ (default) (from_uint_size (seq_len input)) in
+           {a: choice_type}
+           `{Default ((a))}
+           (input: ((seq a)))
+           (start_fin: (((uint_size)) * ((uint_size))))
+  : ((seq a)) :=
+  let out := array_new_ (default) ((seq_len input)) in
   let (start, fin) := start_fin in
-  array_to_seq (update_sub out 0 ((from_uint_size fin) - (from_uint_size start)) ((lseq_slice (array_from_seq (from_uint_size (seq_len input)) input) (from_uint_size start) (from_uint_size fin)))).
+  array_to_seq (update_sub out 0 ((from_uint_size fin) - (from_uint_size start)) ((lseq_slice (array_from_seq ( (seq_len input)) input) (from_uint_size start) (from_uint_size fin)))).
 
-Definition seq_from_seq {A} (l : seq A) : seq A := l.
+Definition seq_from_seq {A} (l : (seq A)) : (seq A) := l.
 
 (**** Chunking *)
 
-Definition seq_num_chunks {a: ChoiceEquality} (s: (T (seq a))) (chunk_len: uint_size) : uint_size :=
+Definition seq_num_chunks {a: choice_type} (s: ((seq a))) (chunk_len: uint_size) : uint_size :=
   ((seq_len s .+ chunk_len .- one) ./ chunk_len)%nat.
 
 Definition seq_chunk_len
-           {a: ChoiceEquality}
-           (s: (T (seq a)))
+           {a: choice_type}
+           (s: ((seq a)))
            (chunk_len: nat)
            (chunk_num: nat)
-  : nat_ChoiceEquality :=
+  : 'nat :=
   let idx_start := (chunk_len * chunk_num)%nat in
   if ((from_uint_size (seq_len s)) <.? (idx_start + chunk_len))%nat then
     ((from_uint_size (seq_len s)) - idx_start)%nat
@@ -1466,41 +1469,41 @@ Definition seq_chunk_len
     chunk_len.
 
 Definition seq_get_chunk
-           {a: ChoiceEquality}
-           `{Default (T (a))}
-           (s: (T (seq a)))
+           {a: choice_type}
+           `{Default ((a))}
+           (s: ((seq a)))
            (chunk_len: uint_size)
            (chunk_num: uint_size)
-  : ((T (uint_size '× seq a)))
+  : (((chProd (uint_size) (seq a))))
   :=
   let idx_start := (from_uint_size chunk_len * from_uint_size chunk_num)%nat in
   let out_len := seq_chunk_len s (from_uint_size chunk_len) (from_uint_size chunk_num) in
-  (usize out_len, array_to_seq (lseq_slice (array_from_seq (from_uint_size (seq_len s)) s) idx_start (idx_start + seq_chunk_len s (from_uint_size chunk_len) (from_uint_size chunk_num)))).
+  (usize out_len, array_to_seq (lseq_slice (array_from_seq ( (seq_len s)) s) idx_start (idx_start + seq_chunk_len s (from_uint_size chunk_len) (from_uint_size chunk_num)))).
 
 Definition seq_set_chunk
-           {a: ChoiceEquality}
-           `{Default (T (a))}
-           (s: (T (seq a)))
+           {a: choice_type}
+           `{Default ((a))}
+           (s: ((seq a)))
            (chunk_len: uint_size)
            (chunk_num: uint_size)
-           (chunk: (T (seq a)) ) : (T (seq a)) :=
+           (chunk: ((seq a)) ) : ((seq a)) :=
   let idx_start := (from_uint_size chunk_len * from_uint_size chunk_num)%nat in
   let out_len := seq_chunk_len s (from_uint_size chunk_len) (from_uint_size chunk_num) in
-  array_to_seq (update_sub (array_from_seq (from_uint_size (seq_len s)) s) idx_start out_len (array_from_seq (from_uint_size (seq_len chunk)) chunk)).
+  array_to_seq (update_sub (array_from_seq ( (seq_len s)) s) idx_start out_len (array_from_seq ( (seq_len chunk)) chunk)).
 
 
-Definition seq_num_exact_chunks {a} (l : (T (seq a))) (chunk_size : (T (uint_size))) : (T (uint_size)) :=
+Definition seq_num_exact_chunks {a} (l : ((seq a))) (chunk_size : ((uint_size))) : ((uint_size)) :=
   (repr (Z.of_nat (length l))) ./ chunk_size.
 
 (* Until #84 is fixed this returns an empty sequence if not enough *)
-Definition seq_get_exact_chunk {a : ChoiceEquality} `{Default (T (a))} (l : (T (seq a))) (chunk_size chunk_num: (T (uint_size))) : (T (seq a)) :=
+Definition seq_get_exact_chunk {a : choice_type} `{Default ((a))} (l : ((seq a))) (chunk_size chunk_num: ((uint_size))) : ((seq a)) :=
   let '(len, chunk) := seq_get_chunk l chunk_size chunk_num in
   if eqtype.eq_op len chunk_size then emptym else chunk.
 
-Definition seq_set_exact_chunk {a : ChoiceEquality} `{H : Default (T (a))} :=
+Definition seq_set_exact_chunk {a : choice_type} `{H : Default ((a))} :=
   @seq_set_chunk a H.
 
-Definition seq_get_remainder_chunk {a : ChoiceEquality} `{Default a} (l : seq a) (chunk_size : uint_size) : seq a :=
+Definition seq_get_remainder_chunk {a : choice_type} `{Default (a)} (l : (seq a)) (chunk_size : uint_size) : (seq a) :=
   let chunks := seq_num_chunks l chunk_size in
   let last_chunk := if (zero <.? chunks)
                     then (chunks .- one)%nat
@@ -1512,14 +1515,14 @@ Definition seq_get_remainder_chunk {a : ChoiceEquality} `{Default a} (l : seq a)
 
 Check @fmap.FMap.FMap _ _ [].
 
-Fixpoint list_xor_ {WS} (x y : list (@int WS)) : list (@int WS) :=
+Fixpoint list_xor_ {WS} (x y : list ((@int WS))) : list ((@int WS)) :=
   match x, y with
   | (x :: xs), (y :: ys) => (int_xor x y) :: (list_xor_ xs ys)
   | [] , _ => y
   | _, [] => x
   end.
 
-Definition seq_xor_ {WS} (x y : seq (@int WS)) : seq (@int WS) :=
+Definition seq_xor_ {WS} (x y : (seq (@int WS))) : (seq (@int WS)) :=
   seq_from_list _ (list_xor_ (seq_to_list _ x) (seq_to_list _ y)).
 Infix "seq_xor" := seq_xor_ (at level 33) : hacspec_scope.
 
@@ -1529,19 +1532,19 @@ Fixpoint list_truncate {a} (x : list a) (n : nat) : list a :=
   | [], _ => []
   | (x :: xs), S n' => x :: (list_truncate xs n')
   end.
-Definition seq_truncate {a} (x : seq a) (n : nat) : seq a :=
+Definition seq_truncate {a} (x : (seq a)) (n : nat) : (seq a) :=
   seq_from_list _ (list_truncate (seq_to_list _ x) n).
 
 (**** Numeric operations *)
 
 (* takes two nseq's and joins them using a function op : a -> a -> a *)
 Definition array_join_map
-           {a: ChoiceEquality}
-           `{Default (T (a))}
+           {a: choice_type}
+           `{Default ((a))}
            {len: nat}
-           (op: (T (a)) -> (T (a)) -> (T (a)))
-           (s1: (T (nseq a len)))
-           (s2 : (T (nseq a len))) :=
+           (op: ((a)) -> ((a)) -> ((a)))
+           (s1: ((nseq' a len)))
+           (s2 : ((nseq' a len))) :=
   let out := s1 in
   foldi (usize 0%nat) (usize len) out (fun i out =>
                                          array_upd out i (op (array_index s1 i) (array_index s2 i))
@@ -1556,11 +1559,11 @@ Infix "array_or" := (array_join_map int_or) (at level 33) : hacspec_scope.
 Infix "array_and" := (array_join_map int_and) (at level 33) : hacspec_scope.
 
 Fixpoint array_eq_
-         {a: ChoiceEquality}
+         {a: choice_type}
          {len: nat}
-         (eq: (T (a)) -> (T (a)) -> bool)
-         (s1: (T (nseq a len)))
-         (s2 : (T (nseq a len)))
+         (eq: ((a)) -> ((a)) -> bool)
+         (s1: ((nseq' a len)))
+         (s2 : ((nseq' a len)))
          {struct len}
   : bool.
 Proof.
@@ -1578,91 +1581,91 @@ Infix "array_neq" := (fun s1 s2 => negb (array_eq_ eq s1 s2)) (at level 33) : ha
 
 
 (**** Integers to arrays *)
-Axiom uint32_to_le_bytes : int32 -> nseq int8 4.
+Axiom uint32_to_le_bytes : int32 -> (nseq int8 (usize 4%nat)).
 (* Definition uint32_to_le_bytes (x: uint32) : nseq uint8 4 :=
   LBSeq.uint_to_bytes_le x. *)
 
-Axiom uint32_to_be_bytes : int32 -> nseq int8 4.
+Axiom uint32_to_be_bytes : int32 -> (nseq int8 (usize 4%nat)).
 (* Definition uint32_to_be_bytes (x: uint32) : nseq uint8 4 :=
   LBSeq.uint_to_bytes_be x *)
 
-Axiom uint32_from_le_bytes : nseq int8 4 -> int32.
+Axiom uint32_from_le_bytes : (nseq int8 (usize 4%nat)) -> int32.
 (* Definition uint32_from_le_bytes (s: nseq uint8 4) : uint32 :=
   LBSeq.uint_from_bytes_le s *)
 
-Axiom uint32_from_be_bytes : nseq int8 4 -> int32.
+Axiom uint32_from_be_bytes : (nseq int8 (usize 4%nat)) -> int32.
 (* Definition uint32_from_be_bytes (s: nseq uint8 4) : uint32 :=
   LBSeq.uint_from_bytes_be s *)
 
-Axiom uint64_to_le_bytes : int64 -> nseq int8 8.
+Axiom uint64_to_le_bytes : int64 -> (nseq int8 (usize 8%nat)).
 (* Definition uint64_to_le_bytes (x: uint64) : nseq uint8 8 :=
   LBSeq.uint_to_bytes_le x *)
 
-Axiom uint64_to_be_bytes : int64 -> nseq int8 8.
+Axiom uint64_to_be_bytes : int64 -> (nseq int8 (usize 8%nat)).
 (* Definition uint64_to_be_bytes (x: uint64) : nseq uint8 8 :=
   LBSeq.uint_to_bytes_be x *)
 
-Axiom uint64_from_le_bytes : nseq int8 8 -> int64.
+Axiom uint64_from_le_bytes : (nseq int8 (usize 8%nat)) -> int64.
 (* Definition uint64_from_le_bytes (s: nseq uint8 8) : uint64 :=
   LBSeq.uint_from_bytes_le s *)
 
-Axiom uint64_from_be_bytes : nseq int8 8 -> int64.
+Axiom uint64_from_be_bytes : (nseq int8 (usize 8%nat)) -> int64.
 (* Definition uint64_from_be_bytes (s: nseq uint8 8) : uint64 :=
   LBSeq.uint_from_bytes_be s *)
 
-Axiom uint128_to_le_bytes : int128 -> nseq int8 16.
+Axiom uint128_to_le_bytes : int128 -> (nseq int8 (usize 16%nat)).
 (* Definition uint128_to_le_bytes (x: uint128) : nseq uint8 16 :=
   LBSeq.uint_to_bytes_le x *)
 
-Axiom uint128_to_be_bytes : int128 -> nseq int8 16.
+Axiom uint128_to_be_bytes : int128 -> (nseq int8 (usize 16%nat)).
 (* Definition uint128_to_be_bytes (x: uint128) : nseq uint8 16 :=
   LBSeq.uint_to_bytes_be x *)
 
-Axiom uint128_from_le_bytes : nseq int8 16 -> int128.
+Axiom uint128_from_le_bytes : (nseq int8 (usize 16%nat)) -> int128.
 (* Definition uint128_from_le_bytes (input: nseq uint8 16) : uint128 :=
   LBSeq.uint_from_bytes_le input *)
 
-Axiom uint128_from_be_bytes : nseq int8 16 -> int128.
+Axiom uint128_from_be_bytes : (nseq int8 (usize 16%nat)) -> int128.
 (* Definition uint128_from_be_bytes (s: nseq uint8 16) : uint128 :=
   LBSeq.uint_from_bytes_be s *)
 
-Axiom u32_to_le_bytes : int32 -> nseq int8 4.
+Axiom u32_to_le_bytes : int32 -> (nseq int8 (usize 4%nat)).
 (* Definition u32_to_le_bytes (x: pub_uint32) : nseq pub_uint8 4 :=
   LBSeq.uint_to_bytes_le x *)
 
-Axiom u32_to_be_bytes : int32 -> nseq int8 4.
+Axiom u32_to_be_bytes : int32 -> (nseq int8 (usize 4%nat)).
 (* Definition u32_to_be_bytes (x: pub_uint32) : nseq pub_uint8 4 :=
   LBSeq.uint_to_bytes_be x *)
 
-Axiom u32_from_le_bytes : nseq int8 4 -> int32.
+Axiom u32_from_le_bytes : (nseq int8 (usize 4%nat)) -> int32.
 (* Definition u32_from_le_bytes (s: nseq pub_uint8 4) : pub_uint32 :=
   LBSeq.uint_from_bytes_le s *)
 
-Axiom u32_from_be_bytes : nseq int8 4 -> int32.
+Axiom u32_from_be_bytes : (nseq int8 (usize 4%nat)) -> int32.
 (* Definition u32_from_be_bytes (s: nseq pub_uint8 4) : pub_uint32 :=
   LBSeq.uint_from_bytes_be s *)
 
-Axiom u64_to_le_bytes : int64 -> nseq int8 8.
+Axiom u64_to_le_bytes : int64 -> (nseq int8 (usize 8%nat)).
 (* Definition u64_to_le_bytes (x: int64) : nseq int8 8 :=
   LBSeq.uint_to_bytes_le x *)
 
-Axiom u64_from_le_bytes : nseq int8 8 -> int64.
+Axiom u64_from_le_bytes : (nseq int8 (usize 8%nat)) -> int64.
 (* Definition u64_from_le_bytes (s: nseq int8 8) : int64 :=
   LBSeq.uint_from_bytes_le s *)
 
-Axiom u128_to_le_bytes : int128 -> nseq int8 16.
+Axiom u128_to_le_bytes : int128 -> (nseq int8 (usize 16%nat)).
 (* Definition u128_to_le_bytes (x: int128) : nseq int8 16 :=
   LBSeq.uint_to_bytes_le x *)
 
-Axiom u128_to_be_bytes : int128 -> nseq int8 16.
+Axiom u128_to_be_bytes : int128 -> (nseq int8 (usize 16%nat)).
 (* Definition u128_to_be_bytes (x: int128) : nseq int8 16 :=
   LBSeq.uint_to_bytes_be x *)
 
-Axiom u128_from_le_bytes : nseq int8 16 -> int128.
+Axiom u128_from_le_bytes : (nseq int8 (usize 16%nat)) -> int128.
 (* Definition u128_from_le_bytes (input: nseq int8 16) : int128 :=
   LBSeq.uint_from_bytes_le input *)
 
-Axiom u128_from_be_bytes : nseq int8 16 -> int128.
+Axiom u128_from_be_bytes : (nseq int8 (usize 16%nat)) -> int128.
 (* Definition u128_from_be_bytes (s: nseq int8 16) : pub_uint128 :=
   LBSeq.uint_from_bytes_be s *)
 
@@ -1670,48 +1673,48 @@ Axiom u128_from_be_bytes : nseq int8 16 -> int128.
 (*** Nats *)
 
 
-Definition nat_mod_choice {p : Z} : choice_type := 'fin (S (Init.Nat.pred (Z.to_nat p))).
+Definition nat_mod(* _choice *) (p : Z) : choice_type := 'fin (S (Init.Nat.pred (Z.to_nat p))).
 Definition nat_mod_type {p : Z} : Type := 'I_(S (Init.Nat.pred (Z.to_nat p))).
-#[global] Instance nat_mod (p : Z) : ChoiceEquality :=
-  {| ct :=  nat_mod_choice ; T :=  @nat_mod_type p ; ChoiceEq := eq_refl |}.
-Definition mk_natmod {p} (z : Z) : nat_mod p := @zmodp.inZp (Init.Nat.pred (Z.to_nat p)) (Z.to_nat z).
+(* #[global] Instance nat_mod (p : Z) : choice_type := *)
+(*   {| ct :=  nat_mod_choice ; :=  @nat_mod_type p ; ChoiceEq := eq_refl |}. *)
+Definition mk_natmod {p} (z : Z) : (nat_mod p) := @zmodp.inZp (Init.Nat.pred (Z.to_nat p)) (Z.to_nat z).
 
 
-Definition nat_mod_equal {p} (a b : nat_mod p) : bool :=
+Definition nat_mod_equal {p} (a b : (nat_mod p)) : bool :=
   @eqtype.eq_op (ordinal_eqType (S (Init.Nat.pred (Z.to_nat p)))) a b.
 
 Definition nat_mod_equal_reflect {p} {a b} : Bool.reflect (a = b) (@nat_mod_equal p a b) :=
   @eqtype.eqP (ordinal_eqType (S (Init.Nat.pred (Z.to_nat p)))) a b.
 
-Definition nat_mod_zero {p} : nat_mod p := zmodp.Zp0.
-Definition nat_mod_one {p} : nat_mod p := zmodp.Zp1.
-Definition nat_mod_two {p} : nat_mod p := zmodp.inZp 2.
+Definition nat_mod_zero {p} : (nat_mod p) := zmodp.Zp0.
+Definition nat_mod_one {p} : (nat_mod p) := zmodp.Zp1.
+Definition nat_mod_two {p} : (nat_mod p) := zmodp.inZp 2.
 
 
 (* convenience coercions from nat_mod to Z and N *)
 (* Coercion Z.of_N : N >-> Z. *)
 
-Definition nat_mod_add {n : Z} (a : nat_mod n) (b : nat_mod n) : nat_mod n := zmodp.Zp_add a b.
+Definition nat_mod_add {n : Z} (a : (nat_mod n)) (b : (nat_mod n)) : (nat_mod n) := zmodp.Zp_add a b.
 
 Infix "+%" := nat_mod_add (at level 33) : hacspec_scope.
 
-Definition nat_mod_mul {n : Z} (a:nat_mod n) (b:nat_mod n) : nat_mod n := zmodp.Zp_mul a b.
+Definition nat_mod_mul {n : Z} (a:(nat_mod n)) (b:(nat_mod n)) : (nat_mod n) := zmodp.Zp_mul a b.
 Infix "*%" := nat_mod_mul (at level 33) : hacspec_scope.
 
-Definition nat_mod_sub {n : Z} (a:nat_mod n) (b:nat_mod n) : nat_mod n := zmodp.Zp_add a (zmodp.Zp_opp b).
+Definition nat_mod_sub {n : Z} (a:(nat_mod n)) (b:(nat_mod n)) : (nat_mod n) := zmodp.Zp_add a (zmodp.Zp_opp b).
 Infix "-%" := nat_mod_sub (at level 33) : hacspec_scope.
 
-Definition nat_mod_div {n : Z} (a:nat_mod n) (b:nat_mod n) : nat_mod n := zmodp.Zp_mul a (zmodp.Zp_inv b).
+Definition nat_mod_div {n : Z} (a:(nat_mod n)) (b:(nat_mod n)) : (nat_mod n) := zmodp.Zp_mul a (zmodp.Zp_inv b).
 Infix "/%" := nat_mod_div (at level 33) : hacspec_scope.
 
 (* A % B = (a * B + r) *)
 
-Definition nat_mod_neg {n : Z} (a:nat_mod n) : nat_mod n := zmodp.Zp_opp a.
+Definition nat_mod_neg {n : Z} (a:(nat_mod n)) : (nat_mod n) := zmodp.Zp_opp a.
 
-Definition nat_mod_inv {n : Z} (a:nat_mod n) : nat_mod n := zmodp.Zp_inv a.
+Definition nat_mod_inv {n : Z} (a:(nat_mod n)) : (nat_mod n) := zmodp.Zp_inv a.
 
-Definition nat_mod_exp_def {p : Z} (a:nat_mod p) (n : nat) : nat_mod p :=
-  let fix exp_ (e : nat_mod p) (n : nat) :=
+Definition nat_mod_exp_def {p : Z} (a:(nat_mod p)) (n : nat) : (nat_mod p) :=
+  let fix exp_ (e : (nat_mod p)) (n : nat) :=
     match n with
     | 0%nat => nat_mod_one
     | S n => nat_mod_mul a (exp_ a n)
@@ -1726,23 +1729,23 @@ Definition nat_mod_pow_self {p} a n := @nat_mod_pow_felem p a n.
 Close Scope nat_scope.
 
 (* We assume x < m *)
-Definition nat_mod_from_secret_literal {m : Z} (x:int128) : nat_mod m := @zmodp.inZp (Init.Nat.pred (Z.to_nat m)) (Z.to_nat (unsigned x)).
+Definition nat_mod_from_secret_literal {m : Z} (x:int128) : (nat_mod m) := @zmodp.inZp (Init.Nat.pred (Z.to_nat m)) (Z.to_nat (unsigned x)).
 
-Definition nat_mod_from_literal (m : Z) (x:int128) : nat_mod m := nat_mod_from_secret_literal x.
+Definition nat_mod_from_literal (m : Z) (x:int128) : (nat_mod m) := nat_mod_from_secret_literal x.
 
-Axiom nat_mod_to_byte_seq_le : forall {n : Z}, nat_mod n -> seq int8.
-Axiom nat_mod_to_byte_seq_be : forall {n : Z}, nat_mod n -> seq int8.
-Axiom nat_mod_to_public_byte_seq_le : forall (n : Z), nat_mod n -> seq int8.
-Axiom nat_mod_to_public_byte_seq_be : forall (n : Z), nat_mod n -> seq int8.
+Axiom nat_mod_to_byte_seq_le : forall {n : Z}, (nat_mod n) -> (seq int8).
+Axiom nat_mod_to_byte_seq_be : forall {n : Z}, (nat_mod n) -> (seq int8).
+Axiom nat_mod_to_public_byte_seq_le : forall (n : Z), (nat_mod n) -> (seq int8).
+Axiom nat_mod_to_public_byte_seq_be : forall (n : Z), (nat_mod n) -> (seq int8).
 
-Definition nat_mod_val (p : Z) (a : nat_mod p) : Z := Z.of_nat (nat_of_ord a).
+Definition nat_mod_val (p : Z) (a : (nat_mod p)) : Z := Z.of_nat (nat_of_ord a).
 
-Definition nat_mod_bit {n : Z} (a : nat_mod n) (i : uint_size) : bool_ChoiceEquality :=
+Definition nat_mod_bit {n : Z} (a : (nat_mod n)) (i : uint_size) : 'bool :=
   Z.testbit (nat_mod_val _ a) (from_uint_size i).
 
 (* Alias for nat_mod_bit *)
-Definition nat_get_mod_bit {p} (a : nat_mod p) := nat_mod_bit a.
-Definition nat_mod_get_bit {p} (a : nat_mod p) n :=
+Definition nat_get_mod_bit {p} (a : (nat_mod p)) := nat_mod_bit a.
+Definition nat_mod_get_bit {p} (a : (nat_mod p)) n :=
   if (nat_mod_bit a n)
   then @nat_mod_one p
   else @nat_mod_zero p.
@@ -1756,21 +1759,21 @@ Definition nat_mod_to_public_byte_seq_le (n: pos)  (len: uint_size) (x: nat_mod_
   Definition n' := n % (pow2 (8 * len)) in
   Lib.ByteSequence.nat_to_bytes_be len n' *)
 
-Axiom array_declassify_eq : forall  {A l}, nseq A l -> nseq A l -> bool_ChoiceEquality.
-Axiom array_to_le_uint32s : forall {A l}, nseq A l -> seq uint32.  (* (l/4) *)
-Axiom array_to_be_uint32s : forall {l}, nseq uint8 l -> seq uint32.  (* (l/4) *)
-Axiom array_to_le_uint64s : forall {A l}, nseq A l -> seq uint64.  (* (l/8) *)
-Axiom array_to_be_uint64s : forall {l}, nseq uint8 l -> seq uint64.  (* (l/8) *)
-Axiom array_to_le_uint128s : forall {A l}, nseq A l -> seq uint128.  (* (l/16) *)
-Axiom array_to_be_uint128s : forall {l}, nseq uint8 l -> seq uint128.  (* (l/16) *)
-Axiom array_to_le_bytes : forall {A l}, nseq A l -> seq uint8.
-Axiom array_to_be_bytes : forall {A l}, nseq A l -> seq uint8.
-Axiom nat_mod_from_byte_seq_le : forall  {A n}, seq A -> nat_mod n.
-Axiom most_significant_bit : forall {m}, nat_mod m -> uint_size -> uint_size.
+Axiom array_declassify_eq : forall  {A l}, (nseq' A l) -> (nseq' A l) -> 'bool.
+Axiom array_to_le_uint32s : forall {A l}, (nseq' A l) -> (seq uint32).  (* (l/4) *)
+Axiom array_to_be_uint32s : forall {l}, (nseq' uint8 l) -> (seq uint32).  (* (l/4) *)
+Axiom array_to_le_uint64s : forall {A l}, (nseq' A l) -> (seq uint64).  (* (l/8) *)
+Axiom array_to_be_uint64s : forall {l}, (nseq' uint8 l) -> (seq uint64).  (* (l/8) *)
+Axiom array_to_le_uint128s : forall {A l}, (nseq' A l) -> (seq uint128).  (* (l/16) *)
+Axiom array_to_be_uint128s : forall {l}, (nseq' uint8 l) -> (seq uint128).  (* (l/16) *)
+Axiom array_to_le_bytes : forall {A l}, (nseq' A l) -> (seq uint8).
+Axiom array_to_be_bytes : forall {A l}, (nseq' A l) -> (seq uint8).
+Axiom nat_mod_from_byte_seq_le : forall  {A n}, (seq A) -> (nat_mod n).
+Axiom most_significant_bit : forall {m}, (nat_mod m) -> (uint_size) -> (uint_size).
 
 
 (* We assume 2^x < m *)
-Definition nat_mod_pow2 (m : Z) (x : N) : nat_mod m := mk_natmod (Z.pow 2 (Z.of_N x)).
+Definition nat_mod_pow2 (m : Z) (x : N) : (nat_mod m) := mk_natmod (Z.pow 2 (Z.of_N x)).
 
 
 Section Casting.
@@ -1813,27 +1816,27 @@ Section Casting.
       cast := Z.of_N
     }.
 
-  Global Instance cast_Z_to_int {WORDSIZE} : Cast Z (@int WORDSIZE) := {
+  Global Instance cast_Z_to_int {WORDSIZE} : Cast Z ((@int WORDSIZE)) := {
       cast n := repr n
     }.
 
-  Global Instance cast_natmod_to_Z {p} : Cast (nat_mod p) Z := {
+  Global Instance cast_natmod_to_Z {p} : Cast ((nat_mod p)) Z := {
       cast n := nat_mod_val _ n
     }.
 
   (* Note: should be aware of typeclass resolution with int/uint since they are just aliases of each other currently *)
-  Global Instance cast_int8_to_uint32 : Cast int8 uint32 := {
+  Global Instance cast_int8_to_uint32 : Cast (int8) (uint32) := {
       cast n := repr (unsigned n)
     }.
-  Global Instance cast_int8_to_int32 : Cast int8 int32 := {
+  Global Instance cast_int8_to_int32 : Cast (int8) (int32) := {
       cast n := repr (signed n)
     }.
 
-  Global Instance cast_uint8_to_uint32 : Cast uint8 uint32 := {
+  Global Instance cast_uint8_to_uint32 : Cast (uint8) (uint32) := {
       cast n := repr (unsigned n)
     }.
 
-  Global Instance cast_int_to_nat `{WS : wsize} : Cast int nat := {
+  Global Instance cast_int_to_nat `{WS : wsize} : Cast (int) nat := {
       cast n := Z.to_nat (@signed WS n)
     }.
 
@@ -1856,144 +1859,144 @@ Section Coercions.
 
   (* Global Coercion repr : Z >-> int_type. *)
 
-  Definition Z_to_int `{WS : wsize} (n : Z) : @int_type WS := repr n.
-  Global Coercion  Z_to_int : Z >-> int_type.
+  Definition Z_to_int `{WS : wsize} (n : Z) : (@int WS) := repr n.
+  Global Coercion  Z_to_int : Z >-> choice.Choice.sort.
 
-  Definition Z_to_uint_size (n : Z) : uint_size_type := repr n.
-  Global Coercion Z_to_uint_size : Z >-> uint_size_type.
-  Definition Z_to_int_size (n : Z) : int_size_type := repr n.
-  Global Coercion Z_to_int_size : Z >-> int_size_type.
+  Definition Z_to_uint_size (n : Z) : uint_size := repr n.
+  Global Coercion Z_to_uint_size : Z >-> choice.Choice.sort.
+  Definition Z_to_int_size (n : Z) : int_size := repr n.
+  Global Coercion Z_to_int_size : Z >-> choice.Choice.sort.
 
-  Definition N_to_int `{WS : wsize} (n : N) : @int_type WS := repr (Z.of_N n).
+  Definition N_to_int `{WS : wsize} (n : N) : (@int WS) := repr (Z.of_N n).
   Global Coercion N.of_nat : nat >-> N.
-  Global Coercion N_to_int : N >-> int_type.
-  Definition N_to_uint_size (n : Z) : uint_size_type := repr n.
-  Global Coercion N_to_uint_size : Z >-> uint_size_type.
-  Definition nat_to_int `{WS : wsize} (n : nat) : @int_type WS := repr (Z.of_nat n).
-  Global Coercion nat_to_int : nat >-> int_type.
+  Global Coercion N_to_int : N >-> choice.Choice.sort.
+  Definition N_to_uint_size (n : Z) : uint_size := repr n.
+  Global Coercion N_to_uint_size : Z >-> choice.Choice.sort.
+  Definition nat_to_int `{WS : wsize} (n : nat) : (@int WS) := repr (Z.of_nat n).
+  Global Coercion nat_to_int : nat >-> choice.Choice.sort.
 
-  Definition uint_size_to_nat (n : uint_size_type) : nat := from_uint_size n.
-  Global Coercion uint_size_to_nat : uint_size_type >-> nat.
+  Definition uint_size_to_nat (n : uint_size) : nat := from_uint_size n.
+  Global Coercion uint_size_to_nat : choice.Choice.sort >-> nat.
 
-  Definition uint_size_to_Z (n : uint_size_type) : Z := from_uint_size n.
-  Global Coercion uint_size_to_Z : uint_size_type >-> Z.
+  Definition uint_size_to_Z (n : uint_size) : Z := from_uint_size n.
+  Global Coercion uint_size_to_Z : choice.Choice.sort >-> Z.
 
-  Definition uint32_to_nat (n : uint32_type) : nat := unsigned n.
-  Global Coercion uint32_to_nat : uint32_type >-> nat.
+  Definition uint32_to_nat (n : uint32) : nat := Z.to_nat (unsigned n).
+  Global Coercion uint32_to_nat : choice.Choice.sort >-> nat.
 
-  Definition int8_to_nat (n : int8_type) : nat := unsigned n.
-  Global Coercion int8_to_nat : int8_type >-> nat.
-  Definition int16_to_nat (n : int16_type) : nat := unsigned n.
-  Global Coercion int16_to_nat : int16_type >-> nat.
-  Definition int32_to_nat (n : int32_type) : nat := unsigned n.
-  Global Coercion int32_to_nat : int32_type >-> nat.
-  Definition int64_to_nat (n : int64_type) : nat := unsigned n.
-  Global Coercion int64_to_nat : int64_type >-> nat.
-  Definition int128_to_nat (n : int128_type) : nat := unsigned n.
-  Global Coercion int128_to_nat : int128_type >-> nat.
+  Definition int8_to_nat (n : int8) : nat := Z.to_nat (unsigned n).
+  Global Coercion int8_to_nat : choice.Choice.sort >-> nat.
+  Definition int16_to_nat (n : int16) : nat := Z.to_nat (unsigned n).
+  Global Coercion int16_to_nat :choice.Choice.sort >-> nat.
+  Definition int32_to_nat (n : int32) : nat := Z.to_nat (unsigned n).
+  Global Coercion int32_to_nat : choice.Choice.sort >-> nat.
+  Definition int64_to_nat (n : int64) : nat := Z.to_nat (unsigned n).
+  Global Coercion int64_to_nat : choice.Choice.sort >-> nat.
+  Definition int128_to_nat (n : int128) : nat := Z.to_nat (unsigned n).
+  Global Coercion int128_to_nat : choice.Choice.sort >-> nat.
 
   (* coercions int8 >-> int16 >-> ... int128 *)
 
-  Definition int8_to_int16 (n : int8_type) : int16_type := repr n.
-  Global Coercion int8_to_int16 : int8_type >-> int16_type.
+  Definition int8_to_int16 (n : int8) : int16 := repr (unsigned n).
+  Global Coercion int8_to_int16 :choice.Choice.sort >-> choice.Choice.sort.
 
-  Definition int8_to_int32 (n : int8_type) : int32_type := repr n.
-  Global Coercion int8_to_int32 : int8_type >-> int32_type.
+  Definition int8_to_int32 (n : int8) : int32 := repr (unsigned n).
+  Global Coercion int8_to_int32 : choice.Choice.sort >-> choice.Choice.sort.
 
-  Definition int16_to_int32 (n : int16_type) : int32_type := repr n.
-  Global Coercion int16_to_int32 : int16_type >-> int32_type.
+  Definition int16_to_int32 (n : int16) : int32 := repr (unsigned n).
+  Global Coercion int16_to_int32 : choice.Choice.sort >-> choice.Choice.sort.
 
-  Definition int32_to_int64 (n : int32_type) : int64_type := repr n.
-  Global Coercion int32_to_int64 : int32_type >-> int64_type.
+  Definition int32_to_int64 (n : int32) : int64 := repr (unsigned n).
+  Global Coercion int32_to_int64 : choice.Choice.sort >-> choice.Choice.sort.
 
-  Definition int64_to_int128 (n : int64_type) : int128_type := repr n.
-  Global Coercion int64_to_int128 : int64_type >-> int128_type.
+  Definition int64_to_int128 (n : int64) : int128 := repr (unsigned n).
+  Global Coercion int64_to_int128 :choice.Choice.sort >-> choice.Choice.sort.
 
-  Definition int32_to_int128 (n : int32_type) : int128_type := repr n.
-  Global Coercion int32_to_int128 : int32_type >-> int128_type.
+  Definition int32_to_int128 (n : int32) : int128 := repr (unsigned n).
+  Global Coercion int32_to_int128 : choice.Choice.sort >-> choice.Choice.sort.
 
-  Definition uint_size_to_int64 (n : uint_size_type) : int64_type := repr n.
-  Global Coercion uint_size_to_int64 : uint_size_type >-> int64_type.
+  Definition uint_size_to_int64 (n : uint_size) : int64 := repr (unsigned n).
+  Global Coercion uint_size_to_int64 : choice.Choice.sort >-> choice.Choice.sort.
 
 
   (* coercions into nat_mod *)
   Definition Z_in_nat_mod {m : Z} (x:Z) : @nat_mod_type m := @mk_natmod m x.
   (* Global Coercion Z_in_nat_mod : Z >-> nat_mod_type. *)
 
-  Definition int_in_nat_mod {m : Z} `{WS : wsize} (x:@int_type WS) : @nat_mod_type m := mk_natmod (unsigned x).
-  Global Coercion int_in_nat_mod : int_type >-> nat_mod_type.
+  Definition int_in_nat_mod {m : Z} `{WS : wsize} (x:(@int WS)) : (@nat_mod m) := mk_natmod (unsigned x).
+  Global Coercion int_in_nat_mod : choice.Choice.sort >-> choice.Choice.sort.
 
-  Definition nat_mod_in_int {m : Z} `{WS : wsize} (x:@nat_mod_type m) : @int_type WS := (repr (nat_mod_val _ x)).
-  Global Coercion nat_mod_in_int : nat_mod_type >-> int_type.
+  Definition nat_mod_in_int {m : Z} `{WS : wsize} (x:@nat_mod_type m) : (@int WS) := (repr (nat_mod_val _ x)).
+  Global Coercion nat_mod_in_int : nat_mod_type >-> choice.Choice.sort.
 
   Definition nat_mod_in_Z {m : Z} `{WS : wsize} (x:@nat_mod_type m) : Z := (nat_mod_val _ x).
   Global Coercion nat_mod_in_Z : nat_mod_type >-> Z.
 
-  Definition uint_size_in_nat_mod (n : uint_size_type) : @nat_mod_type 16 := int_in_nat_mod n.
-  Global Coercion uint_size_in_nat_mod : uint_size_type >-> nat_mod_type.
+  Definition uint_size_in_nat_mod (n : uint_size) : @nat_mod_type 16 := int_in_nat_mod n.
+  Global Coercion uint_size_in_nat_mod : choice.Choice.sort >-> nat_mod_type.
 
 End Coercions.
 
 
 (*** Casting *)
 
-Definition uint128_from_usize (n : uint_size) : int128 := repr n.
-Definition uint64_from_usize (n : uint_size) : int64 := repr n.
-Definition uint32_from_usize (n : uint_size) : int32 := repr n.
-Definition uint16_from_usize (n : uint_size) : int16 := repr n.
-Definition uint8_from_usize (n : uint_size) : int8 := repr n.
+Definition uint128_from_usize (n : uint_size) : int128 := repr (unsigned n).
+Definition uint64_from_usize (n : uint_size) : int64 := repr (unsigned n).
+Definition uint32_from_usize (n : uint_size) : int32 := repr (unsigned n).
+Definition uint16_from_usize (n : uint_size) : int16 := repr (unsigned n).
+Definition uint8_from_usize (n : uint_size) : int8 := repr (unsigned n).
 
-Definition uint128_from_uint8 (n : int8) : int128 := repr n.
-Definition uint64_from_uint8 (n : int8) : int64 := repr n.
-Definition uint32_from_uint8 (n : int8) : int32 := repr n.
-Definition uint16_from_uint8 (n : int8) : int16 := repr n.
-Definition usize_from_uint8 (n : int8) : uint_size := repr n.
+Definition uint128_from_uint8 (n : int8) : int128 := repr (unsigned n).
+Definition uint64_from_uint8 (n : int8) : int64 := repr (unsigned n).
+Definition uint32_from_uint8 (n : int8) : int32 := repr (unsigned n).
+Definition uint16_from_uint8 (n : int8) : int16 := repr (unsigned n).
+Definition usize_from_uint8 (n : int8) : uint_size := repr (unsigned n).
 
-Definition uint128_from_uint16 (n : int16) : int128 := repr n.
-Definition uint64_from_uint16 (n : int16) : int64 := repr n.
-Definition uint32_from_uint16 (n : int16) : int32 := repr n.
-Definition uint8_from_uint16 (n : int16) : int8 := repr n.
-Definition usize_from_uint16 (n : int16) : uint_size := repr n.
+Definition uint128_from_uint16 (n : int16) : int128 := repr (unsigned n).
+Definition uint64_from_uint16 (n : int16) : int64 := repr (unsigned n).
+Definition uint32_from_uint16 (n : int16) : int32 := repr (unsigned n).
+Definition uint8_from_uint16 (n : int16) : int8 := repr (unsigned n).
+Definition usize_from_uint16 (n : int16) : uint_size := repr (unsigned n).
 
-Definition uint128_from_uint32 (n : int32) : int128 := repr n.
-Definition uint64_from_uint32 (n : int32) : int64 := repr n.
-Definition uint16_from_uint32 (n : int32) : int16 := repr n.
-Definition uint8_from_uint32 (n : int32) : int8 := repr n.
-Definition usize_from_uint32 (n : int32) : uint_size := repr n.
+Definition uint128_from_uint32 (n : int32) : int128 := repr (unsigned n).
+Definition uint64_from_uint32 (n : int32) : int64 := repr (unsigned n).
+Definition uint16_from_uint32 (n : int32) : int16 := repr (unsigned n).
+Definition uint8_from_uint32 (n : int32) : int8 := repr (unsigned n).
+Definition usize_from_uint32 (n : int32) : uint_size := repr (unsigned n).
 
-Definition uint128_from_uint64 (n : int64) : int128 := repr n.
-Definition uint32_from_uint64 (n : int64) : int32 := repr n.
-Definition uint16_from_uint64 (n : int64) : int16 := repr n.
-Definition uint8_from_uint64 (n : int64) : int8 := repr n.
-Definition usize_from_uint64 (n : int64) : uint_size := repr n.
+Definition uint128_from_uint64 (n : int64) : int128 := repr (unsigned n).
+Definition uint32_from_uint64 (n : int64) : int32 := repr (unsigned n).
+Definition uint16_from_uint64 (n : int64) : int16 := repr (unsigned n).
+Definition uint8_from_uint64 (n : int64) : int8 := repr (unsigned n).
+Definition usize_from_uint64 (n : int64) : uint_size := repr (unsigned n).
 
-Definition uint64_from_uint128 (n : int128) : int64 := repr n.
-Definition uint32_from_uint128 (n : int128) : int32 := repr n.
-Definition uint16_from_uint128 (n : int128) : int16 := repr n.
-Definition uint8_from_uint128 (n : int128) : int8 := repr n.
-Definition usize_from_uint128 (n : int128) : uint_size := repr n.
+Definition uint64_from_uint128 (n : int128) : int64 := repr (unsigned n).
+Definition uint32_from_uint128 (n : int128) : int32 := repr (unsigned n).
+Definition uint16_from_uint128 (n : int128) : int16 := repr (unsigned n).
+Definition uint8_from_uint128 (n : int128) : int8 := repr (unsigned n).
+Definition usize_from_uint128 (n : int128) : uint_size := repr (unsigned n).
 
 
 Definition uint8_equal : int8 -> int8 -> bool := eqb.
 
-Theorem nat_mod_eqb_spec : forall {p} (a b : nat_mod p), nat_mod_equal a b = true <-> a = b.
+Theorem nat_mod_eqb_spec : forall {p} (a b : (nat_mod p)), nat_mod_equal a b = true <-> a = b.
 Proof.
   symmetry ; exact (ssrbool.rwP nat_mod_equal_reflect).
 Qed.
 
-Global Instance nat_mod_eqdec {p} : EqDec (nat_mod p) := {
+Global Instance nat_mod_eqdec {p} : EqDec ((nat_mod p)) := {
     eqb := nat_mod_equal ;
     eqb_leibniz := nat_mod_eqb_spec;
   }.
 
-Global Instance nat_mod_comparable `{p : Z} : Comparable (nat_mod p) := {
+Global Instance nat_mod_comparable `{p : Z} : Comparable ((nat_mod p)) := {
     ltb a b := Z.ltb (nat_mod_val p a) (nat_mod_val p b);
-    leb a b := if Zeq_bool a b then true else Z.ltb (nat_mod_val p a) (nat_mod_val p b) ;
+    leb a b := if Zeq_bool (nat_mod_val p a) (nat_mod_val p b) then true else Z.ltb (nat_mod_val p a) (nat_mod_val p b) ;
     gtb a b := Z.ltb (nat_mod_val p b) (nat_mod_val p a);
-    geb a b := if Zeq_bool b a then true else Z.ltb (nat_mod_val p b) (nat_mod_val p a) ;
+    geb a b := if Zeq_bool (nat_mod_val p b) (nat_mod_val p a) then true else Z.ltb (nat_mod_val p b) (nat_mod_val p a) ;
   }.
 
-Fixpoint nat_mod_rem_aux {n : Z} (a:nat_mod n) (b:nat_mod n) (f : nat) {struct f} : nat_mod n :=
+Fixpoint nat_mod_rem_aux {n : Z} (a:(nat_mod n)) (b:(nat_mod n)) (f : nat) {struct f} : (nat_mod n) :=
   match f with
   | O => a
   | S f' =>
@@ -2002,10 +2005,10 @@ Fixpoint nat_mod_rem_aux {n : Z} (a:nat_mod n) (b:nat_mod n) (f : nat) {struct f
       else a
   end.
 
-Definition nat_mod_rem {n : Z} (a:nat_mod n) (b:nat_mod n) : nat_mod n :=
+Definition nat_mod_rem {n : Z} (a:(nat_mod n)) (b:(nat_mod n)) : (nat_mod n) :=
   if nat_mod_equal b nat_mod_zero
   then nat_mod_one
-  else nat_mod_rem_aux a b (S (nat_mod_div a b)).
+  else nat_mod_rem_aux a b (S (Z.to_nat (nat_mod_val _ (nat_mod_div a b)))).
 
 Infix "rem" := nat_mod_rem (at level 33) : hacspec_scope.
 
@@ -2093,86 +2096,87 @@ Definition nat_be_range (k : nat) (z : Z) (n : nat) : Z :=
 
 Compute nat_be_range 4 0 300.
 
-Definition u64_to_be_bytes' : int64 -> nseq int8 8 :=
-  fun k => array_from_list (int8) [@nat_to_int U8 (nat_be_range 4 k 7) ;
-                                   @nat_to_int U8(nat_be_range 4 k 6) ;
-                                   @nat_to_int U8 (nat_be_range 4 k 5) ;
-                                   @nat_to_int U8 (nat_be_range 4 k 4) ;
-                                   @nat_to_int U8 (nat_be_range 4 k 3) ;
-                                   @nat_to_int U8 (nat_be_range 4 k 2) ;
-                                   @nat_to_int U8 (nat_be_range 4 k 1) ;
-                                   @nat_to_int U8 (nat_be_range 4 k 0)].
+Definition u64_to_be_bytes' : int64 -> (nseq' int8 8) :=
+  fun k => array_from_list (int8) [@nat_to_int U8 (Z.to_nat (nat_be_range 4 (unsigned k) 7)) ;
+                                   @nat_to_int U8 (Z.to_nat (nat_be_range 4 (unsigned k) 6)) ;
+                                   @nat_to_int U8 (Z.to_nat (nat_be_range 4 (unsigned k) 5)) ;
+                                   @nat_to_int U8 (Z.to_nat (nat_be_range 4 (unsigned k) 4)) ;
+                                   @nat_to_int U8 (Z.to_nat (nat_be_range 4 (unsigned k) 3)) ;
+                                   @nat_to_int U8 (Z.to_nat (nat_be_range 4 (unsigned k) 2)) ;
+                                   @nat_to_int U8 (Z.to_nat (nat_be_range 4 (unsigned k) 1)) ;
+                                   @nat_to_int U8 (Z.to_nat (nat_be_range 4 (unsigned k) 0))].
 
 
 
-Definition u64_from_be_bytes_fold_fun (i : int8) (s : nat_ChoiceEquality '× int64) : nat_ChoiceEquality '× int64 :=
+Definition u64_from_be_bytes_fold_fun (i : int8) (s : (chProd 'nat int64)) : (chProd 'nat int64) :=
   let (n,v) := s in
-  (S n, v .+ (@repr U64 ((int8_to_nat i) * 2 ^ (4 * n)))).
+  (S n, v .+ (@repr U64 ((int8_to_nat i) * 2 ^ (4 * Z.of_nat n)))).
 
-Definition u64_from_be_bytes' : nseq int8 8 -> int64 :=
+Definition u64_from_be_bytes' : (nseq' int8 8) -> int64 :=
    (fun v => snd (List.fold_right u64_from_be_bytes_fold_fun (0%nat, @repr U64 0) (array_to_list v))).
 
-Definition u64_to_be_bytes : int64 -> nseq int8 8 := u64_to_be_bytes'.
-Definition u64_from_be_bytes : nseq int8 8 -> int64 := u64_from_be_bytes'.
+Definition u64_to_be_bytes : int64 -> (nseq' int8 8) := u64_to_be_bytes'.
+Definition u64_from_be_bytes : (nseq' int8 8) -> int64 := u64_from_be_bytes'.
 
 (* Definition nat_mod_to_byte_seq_be : forall {n : Z}, nat_mod n -> seq int8 := *)
 (*   fun k => VectorDef.of_list . *)
 
 (*** Result *)
 
-#[global] #[refine] Instance result (b a : ChoiceEquality) : ChoiceEquality :=
-  {| ct := chSum a b ; T := (a + b)%type |}.
-Proof.
-  intros.
-  cbn.
-  do 2 rewrite ChoiceEq.
-  reflexivity.
-Defined.
+Definition result (b a : choice_type) : choice_type := chSum a b.
+(*   {| ct := chSum a b ; := (a + b)%type |}. *)
+(* Proof. *)
+(*   intros. *)
+(*   cbn. *)
+(*   do 2 rewrite ChoiceEq. *)
+(*   reflexivity. *)
+(* Defined. *)
 
-Definition Ok {a b : ChoiceEquality} : a -> result b a := @inl a b.
-Definition Err {a b : ChoiceEquality} : b -> result b a := @inr a b.
+Definition Ok {a b : choice_type} : a -> (result b a) := @inl (a) (b).
+Definition Err {a b : choice_type} : b -> (result b a) := @inr (a) (b).
 
 Arguments Ok {_ _}.
 Arguments Err {_ _}.
 
-Definition result_unwrap_safe {a b} (x : result b a) `{match x with inl _ => True | inr _ => False end} : a.
+Definition result_unwrap_safe {a b} (x : (result b a)) `{match x with inl _ => True | inr _ => False end} : a.
   destruct x.
-  apply t.
+  apply s.
   contradiction.
 Defined.
 Axiom falso : False. Ltac admit_falso := destruct falso.
-Definition result_unwrap {a b} (x : result b a) : a :=
+Definition result_unwrap {a b} (x : (result b a)) : a :=
   result_unwrap_safe x (H := ltac:(admit_falso)).
 
-Program Definition option_ChoiceEquality (a : ChoiceEquality) :=
-  {| ct := chOption a ; T := option a ; |}.
-Next Obligation.
-  intros.
-  rewrite ChoiceEq.
-  reflexivity.
-Qed.
+Definition option := chOption.
+(* Program Definition option_choice_type (a : choice_type) := *)
+(*   {| ct := chOption a ; := option a ; |}. *)
+(* Next Obligation. *)
+(*   intros. *)
+(*   rewrite ChoiceEq. *)
+(*   reflexivity. *)
+(* Qed. *)
 
 (*** TODO: implement or replace *)
 
 (*** Monad / Bind *)
 
 Module ChoiceEqualityMonad.
-  Class CEMonad (M : ChoiceEquality -> ChoiceEquality) : Type :=
+  Class CEMonad (M : choice_type -> choice_type) : Type :=
     {
-      bind {A B : ChoiceEquality} (x : M A) (f : A -> M B) : M B ;
-      ret {A : ChoiceEquality} (x : A) : M A ;
+      bind {A B : choice_type} (x : (M A)) (f : A -> (M B)) : (M B) ;
+      ret {A : choice_type} (x : A) : (M A) ;
 
-      (* bind_ret : forall {A B : ChoiceEquality} (x : A) (f : A -> M B), bind (ret x) f = f x ; *)
-      (* ret_bind : forall {A : ChoiceEquality} (x : M A) , bind x ret = x ; *)
-      (* bind_cong : forall {A B C : ChoiceEquality} (x : M A) (f : A -> M B) (g : B -> M C), *)
+      (* bind_ret : forall {A B : choice_type} (x : A) (f : A -> M B), bind (ret x) f = f x ; *)
+      (* ret_bind : forall {A : choice_type} (x : M A) , bind x ret = x ; *)
+      (* bind_cong : forall {A B C : choice_type} (x : M A) (f : A -> M B) (g : B -> M C), *)
       (*   bind (bind x f) g = bind x (fun x => bind (f x) g) ; *)
     }.
 
-  Class CEMonad2 (M : ChoiceEquality -> ChoiceEquality) : Type :=
+  Class CEMonad2 (M : choice_type -> choice_type) : Type :=
     {
-      unit {A : ChoiceEquality} (x : A) : M A ;
-      fmap {A B : ChoiceEquality} (f : A -> B) (x : M A) : M B ;
-      join {A : ChoiceEquality} (x : M (M A)) : M A ;
+      unit {A : choice_type} (x : A) : (M A) ;
+      fmap {A B : choice_type} (f : A -> B) (x : (M A)) : (M B) ;
+      join {A : choice_type} (x : (M (M A))) : (M A) ;
     }.
 
   #[global] Instance CEMonadToCEMonad2 `{CEMonad} : CEMonad2 M :=
@@ -2188,8 +2192,8 @@ Module ChoiceEqualityMonad.
       bind A B x f := join (fmap f x)
     |}.
 
-  Class CEMonad_prod (M M0 : ChoiceEquality -> ChoiceEquality) :=
-    { prod : forall A, M0 (M (M0 A)) -> M (M0 A) }.
+  Class CEMonad_prod (M M0 : choice_type -> choice_type) :=
+    { prod : forall A, (M0 (M (M0 A))) -> (M (M0 A)) }.
 
   #[global] Program Instance ComposeProd2 `{CEMonad2} `{CEMonad2} `{@CEMonad_prod M M0} : CEMonad2 (fun x => M (M0 x)) :=
     {|
@@ -2201,14 +2205,14 @@ Module ChoiceEqualityMonad.
   #[global] Instance ComposeProd `{CEMonad} `{CEMonad} `(@CEMonad_prod M M0) : CEMonad (fun x => M (M0 x)) := (@CEMonad2ToCEMonad _ ComposeProd2).
 
   Definition bind_prod `{CEMonad} `{CEMonad} `{@CEMonad_prod M M0}
-             {A B} (x : M (M0 A)) (f : A -> M (M0 B))
-    : M (M0 B) :=
+             {A B} (x : (M (M0 A))) (f : A -> (M (M0 B)))
+    : (M (M0 B)) :=
     (* bind x (fun y => @prod M M0 _ B (bind y (fun y => ret (f y)))). *)
     (@bind (fun x => M (M0 x)) (ComposeProd _) A B x f).
 
 
-  Class CEMonad_swap (M M0 : ChoiceEquality -> ChoiceEquality) :=
-    { swap : forall A, M0 (M A) -> M (M0 A) }.
+  Class CEMonad_swap (M M0 : choice_type -> choice_type) :=
+    { swap : forall A, (M0 (M A)) -> (M (M0 A)) }.
 
   #[global] Program Instance ComposeSwap2 `{CEMonad2 } `{CEMonad2} `{@CEMonad_swap M M0} : CEMonad2 (fun x => M (M0 x)) :=
     {|
@@ -2220,20 +2224,20 @@ Module ChoiceEqualityMonad.
   #[global] Instance ComposeSwap `{CEMonad} `{CEMonad} `(@CEMonad_swap M M0) : CEMonad (fun x => M (M0 x)) := (@CEMonad2ToCEMonad _ ComposeSwap2).
 
   Definition bind_swap `{CEMonad} `{CEMonad} `{@CEMonad_swap M M0}
-             A B (x : M (M0 A)) (f : A -> M (M0 B)) : M (M0 B) :=
+             A B (x : (M (M0 A))) (f : A -> (M (M0 B))) : (M (M0 B)) :=
     (@bind _ (@ComposeSwap M _ M0 _ _) A B x f).
 
 
   Section ResultMonad.
-    Definition result_bind {C A B} (r : result C A) (f : A -> result C B) : result C B :=
+    Definition result_bind {C A B} (r : (result C A)) (f : A -> (result C B)) : (result C B) :=
       match r with
       | inl a => f a
       | inr e => (@Err B C e)
       end.
 
-    Definition result_ret {C A : ChoiceEquality} (a : A) : result C A := Ok a.
+    Definition result_ret {C A : choice_type} (a : A) : (result C A) := Ok a.
 
-    Global Instance result_monad {C : ChoiceEquality} : CEMonad (result C) :=
+    Global Instance result_monad {C : choice_type} : CEMonad (result C) :=
       {|  (* (@result_bind C) (@result_ret C) *)
         bind := (@result_bind C) ;
         ret := (@result_ret C) ;
@@ -2250,18 +2254,18 @@ Module ChoiceEqualityMonad.
 
 
 
-  Definition option_bind {A B} (r : option A) (f : A -> option B) : option B :=
+  Definition option_bind {A B} (r : (option A)) (f : A -> (option B)) : (option B) :=
     match r with
       Some (a) => f a
     | None => None
     end.
 
-  Definition option_ret {A} (a : A) : option A := Some a.
+  Definition option_ret {A : choice_type} (a : A) : (option A) := Some a.
 
-  Global Instance option_monad : CEMonad option_ChoiceEquality :=
-    Build_CEMonad option_ChoiceEquality (@option_bind) (@option_ret).
+  Global Instance option_monad : CEMonad option :=
+    Build_CEMonad option (@option_bind) (@option_ret).
 
-  Definition option_is_none {A} (x : option A) : bool :=
+  Definition option_is_none {A} (x : (option A)) : bool :=
     match x with
     | None => true
     | _ => false
@@ -2281,8 +2285,8 @@ End ChoiceEqualityMonad.
       format " ' x  'm(' v ')'  ⇠  c1  ;;  '//' c2")
     : hacspec_scope.
 
-Definition foldi_bind {A : ChoiceEquality} `{ChoiceEqualityMonad.CEMonad} (a : uint_size) (b : uint_size) (f : uint_size -> A -> M A) (init : M A) : M A :=
-  @foldi (M A) a b init (fun x y => ChoiceEqualityMonad.bind y (f x)).
+Definition foldi_bind {A : choice_type} `{ChoiceEqualityMonad.CEMonad} (a : uint_size) (b : uint_size) (f : uint_size -> A -> (M A)) (init : (M A)) : (M A) :=
+  @foldi ((M A)) a b init (fun x y => ChoiceEqualityMonad.bind y (f x)).
 
 (*** Notation *)
 
@@ -2294,7 +2298,7 @@ Notation "'ifbnd' b 'thenbnd' x 'elsebnd' y '>>' f" := (if b then ChoiceEquality
 Notation "'foldibnd' s 'to' e 'M(' v ')' 'for' z '>>' f" :=
   (Hacspec_Lib_Pre.foldi s e (ChoiceEqualityMonad.ret z) (fun x y => ChoiceEqualityMonad.bind (M := v) y (f x))) (at level 50) : hacspec_scope.
 
-Axiom nat_mod_from_byte_seq_be : forall  {A n}, seq A -> nat_mod n.
+Axiom nat_mod_from_byte_seq_be : forall  {A n}, (seq A) -> (nat_mod n).
 
 (*** Default *)
 
@@ -2308,19 +2312,19 @@ Global Instance N_default : Default N := {
 Global Instance Z_default : Default Z := {
     default := 0%Z
   }.
-Global Instance uint_size_default : Default uint_size := {
+Global Instance uint_size_default : Default (uint_size) := {
     default := zero
   }.
-Global Instance int_size_default : Default int_size := {
+Global Instance int_size_default : Default (int_size) := {
     default := zero
   }.
-Global Instance int_default {WS : wsize} : Default (@int WS) := {
+Global Instance int_default {WS : wsize} : Default ((@int WS)) := {
     default := repr 0
   }.
-Global Instance uint8_default : Default uint8 := _.
-Global Instance nat_mod_default {p : Z} : Default (nat_mod p) := {
+Global Instance uint8_default : Default (uint8) := _.
+Global Instance nat_mod_default {p : Z} : Default ((nat_mod p)) := {
     default := nat_mod_zero
   }.
-Global Instance prod_default {A B : ChoiceEquality} `{Default A} `{Default B} : Default (A '× B) := {
+Global Instance prod_default {A B : choice_type} `{Default (A)} `{Default (B)} : Default ((chProd A B)) := {
     default := (default, default)
   }.
